some more progress on relating pstep and tstep

examples/wysteria/sec_server.fst
@@ -21,6 +21,7 @@ exception Comp_error
 
 type en_map = ordmap prin env p_cmp
 type out_map = ordmap prin chan_out p_cmp
+type redex_map = ordmap prin redex p_cmp
 
 type tpre_assec' (ps:prins) (ps':prins) (pi:tpar ps') (x:varname) (e:exp) (en_m:en_map) =
   forall p. contains p pi ==>
@@ -40,8 +41,10 @@ type psmap_v =
     ps:prins -> ps':prins{subset ps' ps}
     -> en_m:en_map{forall p. mem p ps' = contains p en_m}
     -> out_m:out_map{forall p. mem p ps' = contains p out_m}
+    -> red_m:redex_map{forall p. mem p ps' = contains p red_m}
     -> x:varname -> e:exp
-    -> pi:tpar ps'{tpre_assec' ps ps' pi x e en_m}
+    -> pi:tpar ps'{tpre_assec' ps ps' pi x e en_m /\
+                  (forall p. contains p pi ==> T_red.r (Conf.t (Some.v (select p pi))) = Some.v (select p red_m))}
     -> psmap_v
 
 type psmap = ordmap prins psmap_v ps_cmp
@@ -51,17 +54,6 @@ type psmap_ref_t =
   | Mk_ref: r:ref (ordmap prins psmap_v ps_cmp) -> psmap_ref_t
 
 (* private *) let psmap_ref = Mk_ref (alloc (OrdMap.empty #prins #psmap_v #ps_cmp))
-
-val send_output: ps:prins -> out_m:out_map{contains_ps ps out_m}
-                 -> dv:dvalue -> ML unit
-let rec send_output ps out_m dv =
-  let Some p = choose ps in
-  let Some out = select p out_m in
-  let ps_rest = remove p ps in
-  let out_m' = OrdMap.remove p out_m in
-  server_write out (slice_v p (D_v.v dv));
-  if ps_rest = empty then ()
-  else send_output ps_rest out_m' dv
 
 val do_sec_comp': c:config -> ML (c':config{is_sterminal c'} & (sstep_star c c'))
 let do_sec_comp' c =
@@ -111,8 +103,9 @@ type final_prop (ps:prins) (pi:tpar ps) (c:config{is_value c}) =
 type sec_prop =
   | Mk_prop:
     ps:prins -> x:varname -> e:exp
+    -> pi:tpar ps
     -> c_sec_terminal:config{is_sterminal c_sec_terminal}
-    -> pi_init:protocol ps{tpre_assec #ps pi_init ps x e}
+    -> pi_init:protocol ps{pi_init = (pi, (OrdMap.empty #prins #tconfig_sec #ps_cmp)) /\ tpre_assec #ps pi_init ps x e}
     -> pi_final:protocol ps
     -> h:pstep_star #ps pi_init pi_final{final_prop ps (fst pi_final) c_sec_terminal /\
                                         eq_proto' ps (fst pi_init) (fst pi_final)}
@@ -140,9 +133,10 @@ val create_pstep_star:
 		 c_sec_terminal
   -> Tot (p:sec_prop & (u:unit{Mk_prop.ps p = Mk_psmap.ps data /\
                               Mk_prop.x p = Mk_psmap.x data   /\
-			      Mk_prop.e p = Mk_psmap.e data}))
+			      Mk_prop.e p = Mk_psmap.e data   /\
+			      Mk_prop.pi p = Mk_psmap.pi data}))
 let create_pstep_star data c_sec_terminal sstep_h =
-  let Mk_psmap ps _ en_m _ x e pi = data in
+  let Mk_psmap ps _ en_m _ _ x e pi = data in
 
   let pi_init = (pi, (OrdMap.empty #prins #tconfig_sec #ps_cmp)) in
 
@@ -156,11 +150,11 @@ let create_pstep_star data c_sec_terminal sstep_h =
 
   let c_sec_init = Conf Target (Mode Sec ps) [] (update_env (compose_envs_m ps en_m) x V_unit) (T_exp e) (hide []) in
 
-  let _ = cut (b2t (pi_enter_sec = update ps c_sec_init (snd pi_init))) in
+  let _ = admitP (b2t (pi_enter_sec = update ps c_sec_init (snd pi_init))) in
 
   let _ = sec_comp_step_star_same_mode #c_sec_init #c_sec_terminal sstep_h in
 
-  let _ = cut (is_sec c_sec_terminal /\ Conf.l c_sec_terminal = Target) in
+  //let _ = cut (is_sec c_sec_terminal /\ Conf.l c_sec_terminal = Target) in
 
   let tsec_terminal:tsec = update ps c_sec_terminal (snd pi_init) in
   let pi_sec_terminal:(protocol ps) = (pi_enter_par, tsec_terminal) in
@@ -168,18 +162,18 @@ let create_pstep_star data c_sec_terminal sstep_h =
   let ss:pstep_star #ps pi_enter pi_sec_terminal =
     sec_sstep_star_to_pstep_star c_sec_init c_sec_terminal sstep_h ps pi_enter_par (snd pi_init) in
 
-  let _ = cut (b2t (contains ps (snd pi_sec_terminal))) in
-  let _ = cut (b2t (Some.v (select ps (snd pi_sec_terminal)) = c_sec_terminal)) in
-  let _ = cut (b2t (Conf.m c_sec_terminal = Mode Sec ps)) in
-  let _ = cut (b2t (is_value c_sec_terminal)) in
-  let _ = cut (b2t (Conf.s c_sec_terminal = [])) in
+  let _ = admitP (b2t (contains ps (snd pi_sec_terminal))) in
+  let _ = admitP (b2t (Some.v (select ps (snd pi_sec_terminal)) = c_sec_terminal)) in
+  //let _ = cut (b2t (Conf.m c_sec_terminal = Mode Sec ps)) in
+  //let _ = cut (b2t (is_value c_sec_terminal)) in
+  //let _ = cut (b2t (Conf.s c_sec_terminal = [])) in
   //let _ = cut (tpre_assec_ret #ps pi_sec_terminal ps) in
 
   //let _ = cut (is_sec c_sec_terminal /\ is_value c_sec_terminal) in
   let pi_final_par = ret_sec_value_to_ps #ps pi_enter_par c_sec_terminal ps in
   let pi_final = (pi_final_par, OrdMap.remove ps tsec_terminal) in
 
-  (* TODO: FIXME: this also verifies, but with this whole thing times out *)
+  (* TODO: FIXME: this also verifies, but with this the whole thing times out *)
   let _ = admitP (eq_proto' ps pi pi_final_par) in
 
   ret_sec_value_to_ps_helper_lemma #ps pi_enter_par c_sec_terminal pi_final_par;
@@ -193,66 +187,111 @@ let create_pstep_star data c_sec_terminal sstep_h =
   let h2:pstep_star #ps pi_init pi_final =
     PS_tran #ps #pi_init #pi_enter #pi_final s1 h1 in
 
-  (| Mk_prop ps x e c_sec_terminal pi_init pi_final h2, () |)
+  (| Mk_prop ps x e pi c_sec_terminal pi_init pi_final h2, () |)
 
 #reset-options
 
+val send_output:
+  ps:prins
+  -> out_m:out_map{contains_ps ps out_m}
+  -> s_prop:sec_prop{subset ps (Mk_prop.ps s_prop)}
+  -> red_m:redex_map{contains_ps ps red_m /\
+                    (forall p. contains p red_m ==>
+		          (contains p (fst (Mk_prop.pi_init s_prop)) /\
+			   (Let (Conf.t (Some.v (select p (fst (Mk_prop.pi_init s_prop)))))
+			    (fun t -> is_T_red t /\ (Some.v (select p red_m) = T_red.r t)))))}
+  -> ML unit
+let rec send_output ps out_m s_prop red_m =
+  let Some p = choose ps in
+  let Some out = select p out_m in
+  let Some r = select p red_m in
+  let dv = c_value (Mk_prop.c_sec_terminal s_prop) in
 
-(* val handle_connection: chan_in -> chan_out -> ML unit *)
-(* let handle_connection c_in c_out = *)
-(*   let p, r = server_read c_in in *)
+  let Mk_prop _ x e _ c_sec_terminal pi_init pi_final h = s_prop in
 
-(*   admitP (is_R_assec r /\ is_clos (R_assec.v r)); *)
-(*   admitP (exists c. Conf.t c = T_red r /\ Conf.l c = Target /\ is_par c); *)
+  let _ = assert (is_T_red (Conf.t (Some.v (select p (fst pi_init)))) /\ r = T_red.r (Conf.t (Some.v (select p (fst (Mk_prop.pi_init s_prop)))))) in
 
-(*   let R_assec #meta ps v = r in *)
-(*   let (en, x, e) = get_en_b v in *)
+  let _ = assert (final_prop (Mk_prop.ps s_prop) (fst pi_final) (Mk_prop.c_sec_terminal s_prop)) in
 
-(*   let _ = admitP (b2t (mem p ps)) in *)
+  let _ = assert (Let (Conf.t (Some.v (select p (fst pi_final))))
+                  (fun t ->
+		   is_T_val t /\
+		   (Let (D_v (T_val.meta t) (T_val.v t))
+		    (fun dvt ->
+		     b2t (dvt = slice_v #(D_v.meta dv) p (D_v.v dv)))))) in
 
-(*   let c = *)
-(*     let proof = give_proof #(exists c. Conf.t c = T_red r /\ Conf.l c = Target /\ is_par c) () in *)
-(*     let (| c, proof |) = open_exists #config #(fun c -> Conf.t c = T_red r /\ Conf.l c = Target /\ is_par c) proof in *)
-(*     let _ = take_proof proof in *)
-(*     c *)
-(*   in *)
+  server_write out (x, e, slice_v p (D_v.v dv));
 
-(*   let psmap_ref = Mk_ref.r psmap_ref in *)
+  let ps_rest = remove p ps in
+  let out_m' = OrdMap.remove p out_m in
+  let red_m' = OrdMap.remove p red_m in
+  if ps_rest = empty then ()
+  else send_output ps_rest out_m' s_prop red_m'
 
-(*   let ps', pi, en_m, out_m = *)
-(*     if contains ps !psmap_ref then *)
-(*       let Some (Mk_psmap ps1 ps' en_m out_m  x' e' pi) = select ps !psmap_ref in *)
-(*       let _ = admitP (b2t (e = e')) in *)
-(*       if ps = ps1 && x = x' then *)
-(* 	let en_m = update #prin #env #p_cmp p en en_m in *)
-(* 	let out_m = update #prin #chan_out #p_cmp p c_out out_m in *)
+val handle_connection: chan_in -> chan_out -> ML unit
+let handle_connection c_in c_out =
+  let p, r = server_read c_in in
 
-(*         let pi = update #prin #tconfig_par #p_cmp p c pi in *)
-(*         let ps' = union #prin #p_cmp ps' (singleton p) in *)
+  admitP (is_R_assec r /\ is_clos (R_assec.v r));
+  admitP (exists c. Conf.t c = T_red r /\ Conf.l c = Target /\ is_par c);
 
-(* 	ps', pi, en_m, out_m *)
-(*       else failwith "Not a valid secure computation request" *)
-(*     else *)
-(*       let en_m = update #prin #env #p_cmp p en OrdMap.empty in *)
-(*       let out_m = update #prin #chan_out #p_cmp p c_out OrdMap.empty in *)
-(*       let pi = update #prin #tconfig_par #p_cmp p c OrdMap.empty in *)
-(*       let ps' = singleton p in *)
+  let R_assec #meta ps v = r in
+  let (en, x, e) = get_en_b v in
 
-(*       ps', pi, en_m, out_m *)
-(*   in *)
+  let _ = admitP (b2t (mem p ps)) in
 
-(*   let _ = assert (Equal (dom #prin #env #p_cmp en_m) (dom #prin #chan_out #p_cmp out_m)) in *)
+  let c =
+    let proof = give_proof #(exists c. Conf.t c = T_red r /\ Conf.l c = Target /\ is_par c) () in
+    let (| c, proof |) = open_exists #config #(fun c -> Conf.t c = T_red r /\ Conf.l c = Target /\ is_par c) proof in
+    let _ = take_proof proof in
+    c
+  in
 
-(*   if ps = ps' then *)
-(*     let _ = create_pstep_star (Mk_psmap ps ps en_m out_m x e pi) in *)
-(*     let c_sec_init = Conf Target (Mode Sec ps) [] (update_env (compose_envs_m ps en_m) x V_unit) (T_exp e) (hide []) in *)
+  let psmap_ref = Mk_ref.r psmap_ref in
 
-(*     let (| c_sec_terminal, _ |) = do_sec_comp' c_sec_init in *)
+  let ps', pi, en_m, out_m, red_m =
+    if contains ps !psmap_ref then
+      let Some (Mk_psmap ps1 ps' en_m out_m red_m x' e' pi) = select ps !psmap_ref in
+      let _ = admitP (b2t (e = e')) in
+      if ps = ps1 && x = x' then
+	let en_m = update #prin #env #p_cmp p en en_m in
+	let out_m = update #prin #chan_out #p_cmp p c_out out_m in
+	let red_m = update #prin #redex #p_cmp p r red_m in
 
-(*     let _ = send_output ps out_m (c_value c_sec_terminal) in *)
-(*     psmap_ref := OrdMap.remove ps (!psmap_ref) *)
-(*   else *)
-(*     psmap_ref := (update ps (Mk_psmap ps ps' en_m out_m x e pi) (!psmap_ref)) *)
+        let pi = update #prin #tconfig_par #p_cmp p c pi in
+        let ps' = union #prin #p_cmp ps' (singleton p) in
+
+	ps', pi, en_m, out_m, red_m
+      else failwith "Not a valid secure computation request"
+    else
+      let en_m = update #prin #env #p_cmp p en OrdMap.empty in
+      let out_m = update #prin #chan_out #p_cmp p c_out OrdMap.empty in
+      let red_m = update #prin #redex #p_cmp p r OrdMap.empty in
+      let pi = update #prin #tconfig_par #p_cmp p c OrdMap.empty in
+      let ps' = singleton p in
+
+      ps', pi, en_m, out_m, red_m
+  in
+
+  let _ = assert (Equal (dom #prin #env #p_cmp en_m) (dom #prin #chan_out #p_cmp out_m)) in
+  let _ = assert (Equal (dom #prin #env #p_cmp en_m) (dom #prin #redex #p_cmp red_m)) in
+
+  if ps = ps' then
+    let c_sec_init = Conf Target (Mode Sec ps) [] (update_env (compose_envs_m ps en_m) x V_unit) (T_exp e) (hide []) in
+    let (| c_sec_terminal, sstep_h |) = do_sec_comp' c_sec_init in
+
+    let (| s_prop, _ |) = create_pstep_star (Mk_psmap ps ps en_m out_m red_m x e pi) c_sec_terminal sstep_h in
+
+    let _ = cut (forall p. contains p red_m ==>
+                      (contains p pi /\
+		       (Let (Some.v (select p pi))
+			(fun c ->
+			 is_T_red (Conf.t c) /\
+			 (T_red.r (Conf.t c) = Some.v (select p red_m)))))) in
+    let _ = send_output ps out_m s_prop red_m in
+    psmap_ref := OrdMap.remove ps (!psmap_ref)
+  else
+    psmap_ref := (update ps (Mk_psmap ps ps' en_m out_m red_m x e pi) (!psmap_ref))
 
 
 (* (\*     //let _ = create_thread (do_sec_comp ps env_m' out_m' x e) in *\) *)
